commit

AP/AP/FreshA/Fresh1.lean
@@ -7,9 +7,9 @@ def AStrat.Fresh1 (a : AStrat) (s : State) (fsp : FSP) : Prop :=
   a.WF ∧ s.aForallWinsDisj fsp a ∧ ∀ (d : DStrat), d.WF →
   ∀ s₁ p, (s₁, p) ∈ s.aPtsSimAt ⟨a, d⟩ → p ∉ s.aVisited s₁
 
--- def AStrat.Fresh1Alt (a : AStrat) (s : State) (fsp : FSP) : Prop :=
---   a.WF ∧ ∀ (d : DStrat), d.WF → ∀ n, ∃ s₁, sys.simulate (Strat.f ⟨a, d⟩) s n = (s₁, 0) ∧
---   s₁.aHwsDisj (fsp.offset n |>.insertSet 0 (s.aVisited s₁).toSet)
+def AStrat.Fresh1Alt (a : AStrat) (s : State) (fsp : FSP) : Prop :=
+  a.WF ∧ ∀ (d : DStrat), d.WF → ∀ n, ∃ s₁, sys.simulate (Strat.f ⟨a, d⟩) s n = (s₁, 0) ∧
+  s₁.aHwsDisj (fsp.offset n |>.insertSet 0 # s.aVisited s₁ |>.toSet.erase s₁.aPos)
 
 def aFreshCnd (s : State) (fsp : FSP) (s₁ : State) : Prop :=
   s₁.aHwsDisj # fsp.offset (s₁.diff s) |>.insertSet 0 # s.aVisited s₁ |>.toSet
@@ -48,7 +48,7 @@ theorem AState.exi_aSeek_tr {s P} [hs : AState s]
   simpa [sys.validTr_of_eq_some h₁, h₁]
 
 theorem AState.aPos_ne_of_tr {s s₁ p} [hs : AState s]
-(h : sys.tr s p = some s₁) : s₁.aPos ≠ s.aPos := by
+(h : sys.tr s p = some s₁) : p ≠ s.aPos := by
   rw [tr_eq_some_iff] at h; grind
 
 theorem State.aPos_notMem_of_aWinsDisj {s : State} {fsp a d}
@@ -85,33 +85,54 @@ theorem State.hasTr_of_aHwsDisj {s fsp} [hs : sys.WF s]
 instance {s fsp} : aFresh s fsp |>.WF := by
   unfold aFresh; infer_instance
 
--- theorem State.fresh1_of_alt {s fsp} {a : AStrat} [hs : sys.WF s]
--- (h : a.Fresh1Alt s fsp) : a.Fresh1 s fsp := by
---   rcases h with ⟨ha, h⟩
---   use ha
---   split_ands
---   · intro d hd n
---     specialize h d hd n
---     choose s₁ h₁ h₂ using h
---     use s₁, h₁
---     have hs₁ : sys.WF s₁ := sys.wf_of_simulate_eq h₁
---     replace h₂ := aPos_notMem_of_aHwsDisj h₂
---     simp at h₂
---     simp [FSP.hasLe]
---     exact h₂.2
---   intro d hd s₁ p h₁
---   specialize h d hd
---   rw [mem_aPtsSimAt_iff_simulate_tr] at h₁
---   choose hs₁ n h₁ s₂ h₂ h₃ using h₁
---   simp at h₂ h₃
---   subst h₃
---   specialize h (n + 1)
---   simp [h₁, h₂] at h
---   rw [←AState.aPos_eq_of_tr h₂]
---   replace h := aPos_notMem_of_aHwsDisj h
---   rw [AState.aVisited_eq_of_tr h₂ # sys.reachable_of_simulate_eq h₁] at h
---   simp at h
---   grind
+-- #check 0 #exit
+
+theorem State.fresh1_of_alt {s fsp} {a : AStrat} [hs : sys.WF s]
+(h : a.Fresh1Alt s fsp) : a.Fresh1 s fsp := by
+  rcases h with ⟨ha, h⟩
+  use ha
+  split_ands
+  · intro d hd n
+    specialize h d hd n
+    choose s₁ h₁ h₂ using h
+    use s₁, h₁
+    have hs₁ : sys.WF s₁ := sys.wf_of_simulate_eq h₁
+    replace h₂ := aPos_notMem_of_aHwsDisj h₂
+    simp at h₂
+    simp [FSP.hasLe]
+    exact h₂
+  intro d hd s₁ p h₁
+  specialize h d hd
+  rw [mem_aPtsSimAt_iff_simulate_tr] at h₁
+  choose hs₁ n h₁ s₂ h₂ h₃ using h₁
+  simp at h₂ h₃
+  subst h₃
+  rw [←AState.aPos_eq_of_tr h₂]
+  
+  -- cases n
+  -- ·
+  --   simp at h₁
+  --   simp [h₁]
+  --   exact AState.aPos_ne_of_tr h₂
+  -- nm n
+  -- 
+  -- simp at h₁
+  -- choose s₀ h₁ h₃ using h₁
+  -- 
+  -- have hs₀ : sys.WF s₀ := sys.wf_of_simulate_eq h₁
+  -- replace hs₀ := DState.of_tr' h₃
+  -- simp at h₃
+  -- 
+  -- specialize h n
+  -- simp [h₁] at h
+  -- replace h := DState.aHwsDisj_insert_two_aPos h
+  
+  -- specialize h (n + 1)
+  -- simp [h₁, h₂] at h
+  -- 
+  -- replace h := AState.aHwsDisj_insert_one_aPos h
+  
+  sorry
 
 -- #check 0 #exit
 
